First we need some helper equations.
\begin{align*}
  u &= xy-\frac{\pi}{4} \\
  \sin^2{u} &= \frac{1-\cos{2u}}{2}
      \iff \cos{2u} = 1 - 2\sin^2{u} \\
  2\sin{u}\cos{u} &= \sin{2u} \\
  u' &= xy' + y \\
  \sin^2{u}' &= 2\sin{u}\cos{u}\cdot u' = \sin{2u}(xy'+y) =
      xy'\sin{2u}+y\sin{2u}
\end{align*}
Simplifying $F(x,y)-1 = 0$,
\begin{align*}
  2(y-x)\frac{1-\cos{2u}}{2} &= 1 \\
  (y-x)(1-\cos{2u}) &= 1
\end{align*}
Multiplying out
\begin{align*}
  (y-x)(1-\cos{2u}) &= 1 \\
  y - y\cos{2u} -x + x\cos{2u} &= 1
\end{align*}
Differentiating both sides using above helpers,
\begin{align*}
  y' - y'\cos{2u} + y\sin{2u}\cdot 2u' - 1 + \cos{2u} - x\sin{2u}\cdot 2u' &= 0 \\
  y' - y'\cos{2u} + 2y\sin{(2u)}(y+xy') - 1 + \cos{2u} - 2x\sin{(2u)}(y+xy') &= 0 \\
  y' - y'\cos{2u} + 2y^2\sin^2{u} + 2xyy'\sin{2u} - 1 + \cos{2u}
    +2xy\sin{2u} + 2x^2y'\sin{2u} &= 0
\end{align*}
Grouping $y'$-terms on the left, rest on the right,
\begin{align*}
  y'\left( 1 - \cos{2u} + 2xy\sin{2u} - 2x^2\sin{2u} \right)
    &= -2y^2\sin{2u} + 2xy\sin{2u} + 1 - \cos{2u}
\end{align*}
Dividing and reorganizing using $\cos{2u} = 1 - 2\sin^2{u}$,
\begin{align*}
  y' &= \frac{-2y^2\sin{2u} + 2xy\sin{2u} + 1 - \cos{2u}}
             {1 - \cos{2u} + 2xy\sin{2u} - 2x^2\sin{2u}}
      = \frac{-2y(y-x)\sin{2u} + 1 - 1 + 2\sin^2{u}}
             {1 - 1 + 2\sin^2{u} + x\sin{2u}(2y-2x)}
\end{align*}
Finally, we get the \textit{exact} same result as in 3 (iv).
\begin{align*}
  y' &= \frac{-2y(y-x)\sin{2u} + 2\sin^2{u}}
             {2\sin^2{u} + x\sin{2u}(2y-2x)}
      = \svar{-\frac{y(y-x)\sin{2u} - \sin^2{u}}
                    {x(y-x)\sin{2u} + \sin^2{u}}}
\end{align*}
